kami-rv32im: slightly modified the [p4mm] definition.

Kami/Ex/ProcMemCorrect.v
@@ -5,7 +5,7 @@ Require Import Kami.Syntax Kami.Semantics Kami.RefinementFacts Kami.Renaming Kam
 Require Import Kami.Renaming Kami.Inline Kami.InlineFacts.
 Require Import Kami.Decomposition Kami.Notations Kami.Tactics Kami.ModuleBoundEx.
 Require Import Ex.MemTypes Ex.OneEltFifo Ex.NativeFifo Ex.MemAsync.
-Require Import Ex.SC Ex.ProcDecSC Ex.ProcThreeStage Ex.ProcThreeStDec Ex.ProcFDCorrect.
+Require Import Ex.SC Ex.ProcDecSC Ex.ProcThreeStage Ex.ProcThreeStDec Ex.ProcFetchDecode.
 Require Import Ex.ProcFourStDec.
 Require Import Eqdep.
 
@@ -35,138 +35,156 @@ Section ProcFour.
                                        Expr ty (SyntaxKind (Pc iaddrSize)))
             (isMMIO: IsMMIOT addrSize).
 
-  (* Abstract d2eElt *)
-  Variable (d2eElt: Kind).
-  Variable (d2ePack:
-              forall ty,
-                Expr ty (SyntaxKind (Bit 2)) -> (* opTy *)
-                Expr ty (SyntaxKind (Bit rfIdx)) -> (* dst *)
-                Expr ty (SyntaxKind (Bit addrSize)) -> (* addr *)
-                Expr ty (SyntaxKind (Data dataBytes)) -> (* val1 *)
-                Expr ty (SyntaxKind (Data dataBytes)) -> (* val2 *)
-                Expr ty (SyntaxKind (Data instBytes)) -> (* rawInst *)
-                Expr ty (SyntaxKind (Pc iaddrSize)) -> (* curPc *)
-                Expr ty (SyntaxKind (Pc iaddrSize)) -> (* nextPc *)
-                Expr ty (SyntaxKind Bool) -> (* epoch *)
-                Expr ty (SyntaxKind d2eElt)).
-  Variables
-    (d2eOpType: forall ty, fullType ty (SyntaxKind d2eElt) ->
-                           Expr ty (SyntaxKind (Bit 2)))
-    (d2eDst: forall ty, fullType ty (SyntaxKind d2eElt) ->
-                        Expr ty (SyntaxKind (Bit rfIdx)))
-    (d2eAddr: forall ty, fullType ty (SyntaxKind d2eElt) ->
-                         Expr ty (SyntaxKind (Bit addrSize)))
-    (d2eVal1 d2eVal2: forall ty, fullType ty (SyntaxKind d2eElt) ->
-                                 Expr ty (SyntaxKind (Data dataBytes)))
-    (d2eRawInst: forall ty, fullType ty (SyntaxKind d2eElt) ->
-                            Expr ty (SyntaxKind (Data instBytes)))
-    (d2eCurPc: forall ty, fullType ty (SyntaxKind d2eElt) ->
-                          Expr ty (SyntaxKind (Pc iaddrSize)))
-    (d2eNextPc: forall ty, fullType ty (SyntaxKind d2eElt) ->
-                           Expr ty (SyntaxKind (Pc iaddrSize)))
-    (d2eEpoch: forall ty, fullType ty (SyntaxKind d2eElt) ->
-                          Expr ty (SyntaxKind Bool)).
-
-  (* Abstract f2dElt *)  
-  Variable (f2dElt: Kind).
-  Variable (f2dPack:
-              forall ty,
-                Expr ty (SyntaxKind (Data instBytes)) -> (* rawInst *)
-                Expr ty (SyntaxKind (Pc iaddrSize)) -> (* curPc *)
-                Expr ty (SyntaxKind (Pc iaddrSize)) -> (* nextPc *)
-                Expr ty (SyntaxKind Bool) -> (* epoch *)
-                Expr ty (SyntaxKind f2dElt)).
-  Variables
-    (f2dRawInst: forall ty, fullType ty (SyntaxKind f2dElt) ->
-                            Expr ty (SyntaxKind (Data instBytes)))
-    (f2dCurPc: forall ty, fullType ty (SyntaxKind f2dElt) ->
-                          Expr ty (SyntaxKind (Pc iaddrSize)))
-    (f2dNextPc: forall ty, fullType ty (SyntaxKind f2dElt) ->
-                           Expr ty (SyntaxKind (Pc iaddrSize)))
-    (f2dEpoch: forall ty, fullType ty (SyntaxKind f2dElt) ->
-                          Expr ty (SyntaxKind Bool)).
-
-  Hypotheses (Hf2dRawInst: forall rawInst curPc nextPc epoch,
-                 evalExpr (f2dRawInst _ (evalExpr (f2dPack rawInst curPc nextPc epoch))) =
-                 evalExpr rawInst)
-             (Hf2dCurPc: forall rawInst curPc nextPc epoch,
-                 evalExpr (f2dCurPc _ (evalExpr (f2dPack rawInst curPc nextPc epoch))) =
-                 evalExpr curPc)
-             (Hf2dNextPc: forall rawInst curPc nextPc epoch,
-                 evalExpr (f2dNextPc _ (evalExpr (f2dPack rawInst curPc nextPc epoch))) =
-                 evalExpr nextPc)
-             (Hf2dEpoch: forall rawInst curPc nextPc epoch,
-                 evalExpr (f2dEpoch _ (evalExpr (f2dPack rawInst curPc nextPc epoch))) =
-                 evalExpr epoch).
-
-  (* Abstract e2wElt *)  
-  Variable (e2wElt: Kind).
-  Variable (e2wPack:
-              forall ty,
-                Expr ty (SyntaxKind d2eElt) -> (* decInst *)
-                Expr ty (SyntaxKind (Data dataBytes)) -> (* execVal *)
-                Expr ty (SyntaxKind e2wElt)).
-  Variables
-    (e2wDecInst: forall ty, fullType ty (SyntaxKind e2wElt) ->
-                            Expr ty (SyntaxKind d2eElt))
-    (e2wVal: forall ty, fullType ty (SyntaxKind e2wElt) ->
-                        Expr ty (SyntaxKind (Data dataBytes))).
-
   Variable (init: ProcInit iaddrSize dataBytes rfIdx).
 
-  Definition p4st: Modules :=
-    ProcFourStDec.p4st
-      getOptype getLdDst getLdAddr getLdSrc calcLdAddr
-      getStAddr getStSrc calcStAddr getStVSrc
-      getSrc1 getSrc2 getDst exec getNextPc
-      alignAddr predictNextPc
-      d2ePack d2eOpType d2eDst d2eAddr d2eVal1 d2eVal2
-      d2eRawInst d2eCurPc d2eNextPc d2eEpoch
-      f2dPack f2dRawInst f2dCurPc f2dNextPc f2dEpoch
-      e2wPack e2wDecInst e2wVal init.
+  Section AbsFIFO.
+    
+    (* Abstract d2eElt *)
+    Variable (d2eElt: Kind).
+    Variable (d2ePack:
+                forall ty,
+                  Expr ty (SyntaxKind (Bit 2)) -> (* opTy *)
+                  Expr ty (SyntaxKind (Bit rfIdx)) -> (* dst *)
+                  Expr ty (SyntaxKind (Bit addrSize)) -> (* addr *)
+                  Expr ty (SyntaxKind (Data dataBytes)) -> (* val1 *)
+                  Expr ty (SyntaxKind (Data dataBytes)) -> (* val2 *)
+                  Expr ty (SyntaxKind (Data instBytes)) -> (* rawInst *)
+                  Expr ty (SyntaxKind (Pc iaddrSize)) -> (* curPc *)
+                  Expr ty (SyntaxKind (Pc iaddrSize)) -> (* nextPc *)
+                  Expr ty (SyntaxKind Bool) -> (* epoch *)
+                  Expr ty (SyntaxKind d2eElt)).
+    Variables
+      (d2eOpType: forall ty, fullType ty (SyntaxKind d2eElt) ->
+                             Expr ty (SyntaxKind (Bit 2)))
+      (d2eDst: forall ty, fullType ty (SyntaxKind d2eElt) ->
+                          Expr ty (SyntaxKind (Bit rfIdx)))
+      (d2eAddr: forall ty, fullType ty (SyntaxKind d2eElt) ->
+                           Expr ty (SyntaxKind (Bit addrSize)))
+      (d2eVal1 d2eVal2: forall ty, fullType ty (SyntaxKind d2eElt) ->
+                                   Expr ty (SyntaxKind (Data dataBytes)))
+      (d2eRawInst: forall ty, fullType ty (SyntaxKind d2eElt) ->
+                              Expr ty (SyntaxKind (Data instBytes)))
+      (d2eCurPc: forall ty, fullType ty (SyntaxKind d2eElt) ->
+                            Expr ty (SyntaxKind (Pc iaddrSize)))
+      (d2eNextPc: forall ty, fullType ty (SyntaxKind d2eElt) ->
+                             Expr ty (SyntaxKind (Pc iaddrSize)))
+      (d2eEpoch: forall ty, fullType ty (SyntaxKind d2eElt) ->
+                            Expr ty (SyntaxKind Bool)).
 
-  Definition iom: Modules :=
-    MemAsync.iom addrSize fifoSize dataBytes.
+    (* Abstract f2dElt *)  
+    Variable (f2dElt: Kind).
+    Variable (f2dPack:
+                forall ty,
+                  Expr ty (SyntaxKind (Data instBytes)) -> (* rawInst *)
+                  Expr ty (SyntaxKind (Pc iaddrSize)) -> (* curPc *)
+                  Expr ty (SyntaxKind (Pc iaddrSize)) -> (* nextPc *)
+                  Expr ty (SyntaxKind Bool) -> (* epoch *)
+                  Expr ty (SyntaxKind f2dElt)).
+    Variables
+      (f2dRawInst: forall ty, fullType ty (SyntaxKind f2dElt) ->
+                              Expr ty (SyntaxKind (Data instBytes)))
+      (f2dCurPc: forall ty, fullType ty (SyntaxKind f2dElt) ->
+                            Expr ty (SyntaxKind (Pc iaddrSize)))
+      (f2dNextPc: forall ty, fullType ty (SyntaxKind f2dElt) ->
+                             Expr ty (SyntaxKind (Pc iaddrSize)))
+      (f2dEpoch: forall ty, fullType ty (SyntaxKind f2dElt) ->
+                            Expr ty (SyntaxKind Bool)).
 
-  Definition p4stf: Modules :=
-    (p4st ++ iom)%kami.
+    Hypotheses (Hf2dRawInst: forall rawInst curPc nextPc epoch,
+                   evalExpr (f2dRawInst _ (evalExpr (f2dPack rawInst curPc nextPc epoch))) =
+                   evalExpr rawInst)
+               (Hf2dCurPc: forall rawInst curPc nextPc epoch,
+                   evalExpr (f2dCurPc _ (evalExpr (f2dPack rawInst curPc nextPc epoch))) =
+                   evalExpr curPc)
+               (Hf2dNextPc: forall rawInst curPc nextPc epoch,
+                   evalExpr (f2dNextPc _ (evalExpr (f2dPack rawInst curPc nextPc epoch))) =
+                   evalExpr nextPc)
+               (Hf2dEpoch: forall rawInst curPc nextPc epoch,
+                   evalExpr (f2dEpoch _ (evalExpr (f2dPack rawInst curPc nextPc epoch))) =
+                   evalExpr epoch).
 
-  Definition pinst: Modules :=
-    SC.pinst
-      getOptype getLdDst getLdAddr getLdSrc calcLdAddr
-      getStAddr getStSrc calcStAddr getStVSrc
-      getSrc1 getSrc2 getDst exec getNextPc
-      alignAddr init.
+    (* Abstract e2wElt *)  
+    Variable (e2wElt: Kind).
+    Variable (e2wPack:
+                forall ty,
+                  Expr ty (SyntaxKind d2eElt) -> (* decInst *)
+                  Expr ty (SyntaxKind (Data dataBytes)) -> (* execVal *)
+                  Expr ty (SyntaxKind e2wElt)).
+    Variables
+      (e2wDecInst: forall ty, fullType ty (SyntaxKind e2wElt) ->
+                              Expr ty (SyntaxKind d2eElt))
+      (e2wVal: forall ty, fullType ty (SyntaxKind e2wElt) ->
+                          Expr ty (SyntaxKind (Data dataBytes))).
 
-  Definition mm: Modules :=
-    SC.mm dataBytes isMMIO.
+    Definition p4st: Modules :=
+      ProcFourStDec.p4st
+        getOptype getLdDst getLdAddr getLdSrc calcLdAddr
+        getStAddr getStSrc calcStAddr getStVSrc
+        getSrc1 getSrc2 getDst exec getNextPc
+        alignAddr predictNextPc
+        d2ePack d2eOpType d2eDst d2eAddr d2eVal1 d2eVal2
+        d2eRawInst d2eCurPc d2eNextPc d2eEpoch
+        f2dPack f2dRawInst f2dCurPc f2dNextPc f2dEpoch
+        e2wPack e2wDecInst e2wVal init.
+
+    Definition iom: Modules :=
+      MemAsync.iom addrSize fifoSize dataBytes.
+
+    Definition p4stf: Modules :=
+      (p4st ++ iom)%kami.
+
+    Definition pinst: Modules :=
+      SC.pinst
+        getOptype getLdDst getLdAddr getLdSrc calcLdAddr
+        getStAddr getStSrc calcStAddr getStVSrc
+        getSrc1 getSrc2 getDst exec getNextPc
+        alignAddr init.
+
+    Definition mm: Modules :=
+      SC.mm dataBytes isMMIO.
+
+    Definition p4mma: Modules :=
+      (p4stf ++ mm)%kami.
+
+    Definition scmm: Modules :=
+      SC.scmm
+        getOptype getLdDst getLdAddr getLdSrc calcLdAddr
+        getStAddr getStSrc calcStAddr getStVSrc
+        getSrc1 getSrc2 getDst exec getNextPc
+        alignAddr isMMIO init.
+    
+    Lemma p4stf_refines_pinst: p4stf <<== pinst.
+    Proof.
+      intros.
+      ketrans; [|apply pdec_refines_pinst].
+      kmodular.
+      - ketrans; [apply p4st_refines_p3st|].
+        apply p3st_refines_pdec.
+      - krefl.
+    Qed.
+
+    Lemma p4mma_correct: p4mma <<== scmm.
+    Proof.
+      intros.
+      kmodular.
+      - apply p4stf_refines_pinst.
+      - krefl.
+    Qed.
+
+  End AbsFIFO.
 
   Definition p4mm: Modules :=
-    (p4stf ++ mm)%kami.
+    p4mma
+      (@d2ePackI _ _ _ _ _) (@d2eOpTypeI _ _ _ _ _) (@d2eDstI _ _ _ _ _) (@d2eAddrI _ _ _ _ _)
+      (@d2eVal1I _ _ _ _ _) (@d2eVal2I _ _ _ _ _) (@d2eRawInstI _ _ _ _ _) (@d2eCurPcI _ _ _ _ _)
+      (@d2eNextPcI _ _ _ _ _) (@d2eEpochI _ _ _ _ _)
+      (@f2dPackI _ _) (@f2dRawInstI _ _) (@f2dCurPcI _ _)
+      (@f2dNextPcI _ _) (@f2dEpochI _ _)
+      (@e2wPackI _ _ _ _ _) (@e2wDecInstI _ _ _ _ _) (@e2wValI _ _ _ _ _).
 
-  Definition scmm: Modules :=
-    SC.scmm
-      getOptype getLdDst getLdAddr getLdSrc calcLdAddr
-      getStAddr getStSrc calcStAddr getStVSrc
-      getSrc1 getSrc2 getDst exec getNextPc
-      alignAddr isMMIO init.
-  
-  Lemma p4stf_refines_pinst: p4stf <<== pinst.
+  Theorem p4mm_correct: p4mm <<== scmm.
   Proof.
-    intros.
-    ketrans; [|apply pdec_refines_pinst].
-    kmodular.
-    - ketrans; [apply p4st_refines_p3st|].
-      apply p3st_refines_pdec.
-    - krefl.
-  Qed.
-
-  Lemma proc_mem_correct: p4mm <<== scmm.
-  Proof.
-    intros.
-    kmodular.
-    - apply p4stf_refines_pinst.
-    - krefl.
+    intros; apply p4mma_correct.
   Qed.
 
 End ProcFour.
